Almost done

code/semantics.v
@@ -1,5 +1,7 @@
 Set Implicit Arguments.
 
+Hint Extern 1 (_ = _) => congruence.
+
 (* syntax *)
 
 Inductive exp : Set :=
@@ -161,6 +163,101 @@ Proof.
     inverts H' ; f_equal ; try repeat s ; auto ; try repeat s1.
 Qed.
 
+Reserved Notation "e '==>*' e1" (at level 40).
+
+Inductive multi_step : exp -> exp -> Prop :=
+| mstep_refl
+  : forall e, e ==>* e
+| mstep_step
+  : forall e e1 e',
+    e ==> e1   ->
+    e1 ==>* e' ->
+    e ==>* e'
+where "e '==>*' e1" := (multi_step e e1).
+
+Hint Constructors multi_step.
+
+Lemma succ_multi_step : forall e e', e ==>* e' -> Succ e ==>* Succ e'.
+Proof.
+  induction 1 ;
+     try match goal with
+         | [H : ?e ==> ?e1, IH : Succ ?e1 ==>* Succ ?e' |- _] =>
+           apply ST_Succ in H ; eapply mstep_step with (e1 := Succ e1) 
+         end ; auto.
+Qed.
+  
+Hint Resolve succ_multi_step.
+
+Reserved Notation "e '==>>' e1" (at level 40).
+
+Inductive big_step : exp -> exp -> Prop :=
+| B_Value
+  : forall v, value v -> v ==>> v
+| B_If_True
+  : forall e e1 e11 e2,
+    e ==>> T ->
+    e1 ==>> e11 ->
+    (If e e1 e2) ==>> e11
+| B_If_False
+  : forall e e1 e2 e22,
+    e ==>> F ->
+    e2 ==>> e22 ->
+    (If e e1 e2) ==>> e22
+| B_Succ
+  : forall e nv,
+    nvalue nv ->
+    e ==>> nv ->
+    (Succ e) ==>> (Succ nv)
+| B_PredZero
+  : forall e,
+    e ==>> Zero ->
+    (Pred e) ==>> Zero
+| B_PredSucc
+  : forall e nv,
+    nvalue nv ->
+    e ==>> (Succ nv) ->
+    Pred e ==>> nv
+| B_IsZeroZero
+  : forall e,
+    e ==>> Zero ->
+    (IsZero e) ==>> T
+| B_IsZeroSucc
+  : forall e nv,
+    nvalue nv ->
+    e ==>> (Succ nv) ->
+    (IsZero e) ==>> F
+where "e '==>>' e1" := (big_step e e1).
+
+Hint Constructors big_step.
+
+Ltac bs := match goal with
+            | [H : T ==>> _ |- _] => inverts H
+            | [H : F ==>> _ |- _] => inverts H                                                
+            | [H : Zero ==>> _ |- _] => inverts H
+            | [H : (Succ _) ==>> _ |- _] => inverts H
+            | [H : value _ |- _] => inverts H
+            | [H : bvalue (Succ _) |- _] => inverts H
+            | [H : nvalue (Succ _) |- _] => inverts H
+            | [H : (Pred _) ==>> _ |- _] => inverts H     
+            | [H : bvalue (Pred _) |- _] => inverts H
+            | [H : nvalue (Pred _) |- _] => inverts H
+            | [H : (If _ _ _) ==>> _ |- _] => inverts H     
+            | [H : bvalue (If _ _ _) |- _] => inverts H
+            | [H : nvalue (If _ _ _) |- _] => inverts H
+            | [H : (IsZero _) ==>> _ |- _] => inverts H     
+            | [H : bvalue (IsZero _) |- _] => inverts H
+            | [H : nvalue (IsZero _) |- _] => inverts H
+            | [ IH : forall v, ?e ==>> v -> forall v', ?e ==>> v' -> _
+                , H : ?e ==>> _, H1 : ?e ==>> _ |- _] =>
+              apply (IH _ H) in H1
+            end ; subst ; try f_equal ; auto.
+  
+
+Lemma big_step_deterministic : forall e v, e ==>> v -> forall v', e ==>> v' -> v = v'.
+Proof.
+  induction e ; intros ; repeat bs.
+Qed.
+
 
 (* typing *)
 
@@ -237,19 +334,6 @@ Proof.
                 end).
 Qed.
 
-Reserved Notation "e '==>*' e1" (at level 40).
-
-Inductive multi_step : exp -> exp -> Prop :=
-| mstep_refl
-  : forall e, e ==>* e
-| mstep_step
-  : forall e e1 e',
-    e ==> e1   ->
-    e1 ==>* e' ->
-    e ==>* e'
-where "e '==>*' e1" := (multi_step e e1).
-
-Hint Constructors multi_step.
 
 
 (* notations for subset types -- sig types *)
@@ -273,11 +357,10 @@ Notation "x <-- e1 ; e2" := (match e1 with
                                | inright _ => !!
                                | inleft (exist _ x _) => e2
                              end)
-                             (right associativity, at level 60).
+                              (right associativity, at level 60).
 
 Notation "e1 ;;; e2" := (if e1 then e2 else !!)
                           (right associativity, at level 60).
-
 
 Definition eq_ty_dec : forall (t t' : type), {t = t'} + {t <> t'}.
   decide equality.
@@ -296,52 +379,25 @@ Definition typecheck : forall e, {t | e <<- t} + {forall t, ~ (e <<- t)}.
             | T  => fun _ => [|| TBool ||]
             | F  => fun _ => [|| TBool ||]
             | Zero  => fun _ => [|| TNat ||]
-            | Succ e => fun _ => 
-              match tc e with
-              | [|| t ||] => 
-                  match eq_ty_dec t TNat with
-                  | Yes => [|| TNat ||]
-                  | No  => !!           
-                  end
-              | !! => !!
-              end          
+            | Succ e => fun _ =>
+                          ty <-- tc e ;
+                          eq_ty_dec ty TNat ;;;
+                          [|| TNat ||]          
             | Pred e => fun _ => 
-              match tc e with
-              | [|| t ||] => 
-                  match eq_ty_dec t TNat with
-                  | Yes => [|| TNat ||]
-                  | No  => !!           
-                  end
-              | !! => !!
-              end          
+                          ty <-- tc e ;
+                          eq_ty_dec ty TNat ;;;
+                          [|| TNat ||]          
             | IsZero e => fun _ => 
-              match tc e with
-              | [|| t ||] =>
-                  match eq_ty_dec t TNat with
-                  | Yes => [|| TBool ||]
-                  | No  => !!           
-                  end
-              | !! => !!
-              end          
-              | If e e1 e2 => fun _ => 
-                match tc e with
-                | [|| t ||] =>
-                  match eq_ty_dec t TBool with
-                  | Yes =>
-                    match tc e1 , tc e2 with
-                    | [|| t1 ||] , [|| t2 ||] =>
-                      match eq_ty_dec t1 t2 with
-                      | Yes => [|| t1 ||]
-                      | No  => !!           
-                      end
-                    | !! , [|| t2 ||] => !!
-                    | [|| t1 ||] , !! => !!
-                    | !! , !! => !!                       
-                    end  
-                  | No  => !!  
-                  end
-                | !! => !!    
-                end    
+                          ty <-- tc e ;
+                          eq_ty_dec ty TNat ;;;
+                          [|| TBool ||]          
+            | If e e1 e2 => fun _ =>
+                          ty <-- tc e ;
+                          ty1 <-- tc e1 ;
+                          ty2 <-- tc e2 ;
+                          eq_ty_dec ty TBool ;;;
+                          eq_ty_dec ty1 ty2  ;;;          
+                          [|| ty1 ||]
             end eq_refl) ; clear tc ;
            simpl in * ; subst ;
              try (intro ; intro) ;
